src/simple-proof/proof/OperationalSemantics.v
@@ -8,6 +8,26 @@ Require Import Definitions Binding.
 
 Reserved Notation "t1 '|->' t2" (at level 40, t2 at level 39).
 
+Fixpoint defs_update (ds: defs) (a: trm_label) (t: trm) : defs :=
+  match ds with
+  | defs_nil => defs_nil
+  | defs_cons ds' (def_typ A T)  =>
+    defs_cons (defs_update ds' a t) (def_typ A T)
+  | defs_cons ds' (def_trm a' t')  =>
+    If a = a' then defs_cons ds' (def_trm a t) else defs_cons (defs_update ds' a t) (def_trm a' t')
+end.
+
+Definition sto_update (x : var) (m : trm_label) (t : trm) (s1 : sta) (s2 : sta) : Prop :=
+    ok s1 /\
+    ok s2 /\
+    dom s1 = dom s2 /\
+    (forall y, (y <> x) ->
+         (forall v, binds y v s1 -> binds y v s2) /\
+         (forall v, binds y v s2 -> binds y v s1)) /\
+    (exists T ds1 ds2, binds x (val_obj T ds1) s1 /\
+                  binds x (val_obj T ds2) s2 /\
+                  defs_update (open_defs x ds1) m t = open_defs x ds2).
+
 Inductive red : sta * trm -> sta * trm -> Prop :=
 (** [s(x) = nu(T)...{a = t}...]  #<br>#
     [―――――――――――――――――――――――――]  #<br>#
@@ -15,7 +35,18 @@ Inductive red : sta * trm -> sta * trm -> Prop :=
 | red_sel : forall x m s t T ds,
     binds x (val_obj T ds) s ->
     defs_has (open_defs x ds) (def_trm m t) ->
-    (s, trm_sel (avar_f x) m) |-> (s, t)
+    (s, trm_sel (avar_f x) m) |-> (s, trm_force (avar_f x) m)
+
+| red_force_loc : forall x m s y T ds,
+    binds x (val_obj T ds) s ->
+    defs_has (open_defs x ds) (def_trm m (trm_var (avar_f y))) ->
+    (s, trm_force (avar_f x) m) |-> (s, (trm_var (avar_f y)))
+
+| red_force_term : forall x m s t T ds,
+    binds x (val_obj T ds) s ->
+    defs_has (open_defs x ds) (def_trm m t) ->
+    (forall y, (trm_var (avar_f y)) <> t) ->
+    (s, trm_force (avar_f x) m) |-> (s, trm_force_assgn (avar_f x) m t)
 
 (** [s(x) = lambda(T)t]      #<br>#
     [―――――――――――――――――――――]  #<br>#
@@ -39,6 +70,15 @@ Inductive red : sta * trm -> sta * trm -> Prop :=
 | red_let_tgt : forall t0 t s t0' s',
     (s, t0) |-> (s', t0') ->
     (s, trm_let t0 t) |-> (s', trm_let t0' t)
+
+| red_force_assgn_trm : forall t0 x m s t0' s',
+    (s, t0) |-> (s', t0') ->
+    (s, trm_force_assgn (avar_f x) m t0) |-> (s, trm_force_assgn (avar_f x) m t0')
+
+| red_force_assgn_var : forall s x m y s',
+    sto_update x m (trm_var (avar_f y)) s s' ->
+    (s, trm_force_assgn (avar_f x) m (trm_var (avar_f y))) |->
+    (s', (trm_var (avar_f y)))
 
 where "t1 '|->' t2" := (red t1 t2).
 
