src/simple-proof/proof/Safety.v
@@ -75,10 +75,140 @@ Ltac solve_IH :=
   match goal with
   | [Hi: _ & ?G' ⊢ _ : _ |- _] =>
     exists G'; repeat_split_right; auto
+  | [Hi: ty_trm_aux (_ & ?G') _ _ |- _] =>
+    exists G'; repeat_split_right; auto
   end.
 
 Ltac solve_let :=
-  invert_red; trm_val_contra; solve_IH; fresh_constructor; eauto; apply* weaken_rules.
+  invert_red; trm_val_contra; solve_IH;
+  apply_fresh ty_aux_let as z; eauto; apply* weaken_rules.
+
+Lemma sel_to_var_typ: forall G x a T,
+  G ⊢ trm_sel (avar_f x) a : T ->
+  G ⊢ trm_var (avar_f x) : typ_rcd (dec_trm a T).
+Proof.
+  introv Hty.
+  dependent induction Hty; auto.
+  eapply ty_sub; eauto.
+Qed.
+
+Lemma record_has_typing: forall G x T d,
+  G ⊢ trm_var (avar_f x) : T ->
+  record_has T d ->
+  G ⊢ trm_var (avar_f x) : typ_rcd d.
+Proof.
+  introv Ht Hr.
+  dependent induction Hr; eauto.
+Qed.
+
+Lemma var_aux_to_gen : forall G y T,
+  ty_trm_aux G (trm_var (avar_f y)) T ->
+  G ⊢ (trm_var (avar_f y)) : T.
+Proof.
+  introv Ht.
+  dependent induction Ht; eauto.
+Qed.
+
+Lemma defs_update_hasnt : forall ds l a t,
+    defs_hasnt ds l ->
+    defs_hasnt (defs_update ds a t) l.
+Proof.
+  induction ds.
+  - intros.
+    simpl; auto.
+  - intros.
+    unfold defs_hasnt in *.
+    simpl in *.
+    cases_if.
+    specialize (IHds l a t H).
+    destruct d.
+    + simpl in *. cases_if. auto.
+    + cases_if. simpl in *; cases_if; auto.
+      simpl in *; cases_if; auto.
+Qed.
+
+Lemma defs_update_typing : forall T a y ds G D,
+  record_has T (dec_trm a D) ->
+  G /- ds :: T ->
+  G ⊢ trm_var (avar_f y) : D ->
+  G /- (defs_update ds a (trm_var (avar_f y))) :: T.
+Proof.
+  induction T; introv Hrh Hds Hty;
+  try solve [inversion Hrh].
+  - inversions Hrh.
+    inversions Hds.
+    inversions H2.
+    simpl. cases_if.
+    auto.
+  - inversions Hds.
+    inversions H4.
+    + simpl.
+      apply ty_defs_cons; auto.
+      inversions Hrh; eauto.
+      inversion H3.
+      eauto using defs_update_hasnt.
+    + pose proof (ty_defs_record_type H1) as [?ls ?].
+      simpl in *. cases_if.
+      { inversions Hrh.
+        pose proof (record_typ_has_label_in H0 H6).
+        pose proof (hasnt_notin H1 H0 H5).
+        simpl in H2.
+        contradiction.
+        inversions H6.
+        pose proof (IHT2 a0 y (defs_cons defs_nil (def_trm a0 (trm_var (avar_f y)))) G D
+                         (rh_one _)
+                         (ty_defs_one (ty_def_trm _ Hty))
+                         Hty
+                   ).
+        simpl in H2; cases_if.
+        inversions H2.
+        apply ty_defs_cons; auto.
+      }
+      { apply ty_defs_cons.
+        eapply IHT1; eauto.
+        inversion Hrh; eauto.
+        inversion H6. exfalso; auto.
+        eauto.
+        eauto using defs_update_hasnt.
+      }
+Qed.
+
+Lemma binds_middle: forall A (E : env A) x v,
+    binds x v E ->
+    exists E1 E2, E = E1 & x ~ v & E2.
+Proof.
+  intros A E. induction E using env_ind.
+  - intros. exfalso. apply (binds_empty_inv H).
+  - introv Bis. apply binds_push_inv in Bis.
+    destruct Bis as [[? ?] | [? ?]].
+    + subst. exists E (@empty A).
+      rewrite concat_empty_r; reflexivity.
+    + pose proof (IHE _ _ H0) as [?E [?E ?]].
+      subst E. exists E0 (E1 & x ~ v).
+      rewrite concat_assoc; auto.
+Qed.
+
+Lemma defs_update_val_typing : forall L ds G a S T x y ds',
+    ok G ->
+    binds x (typ_bnd S) G ->
+    (forall y, y \notin L -> G & (y ~ open_typ y S) /- open_defs y ds :: open_typ y S) ->
+    record_has (open_typ x S) (dec_trm a T) ->
+    defs_update (open_defs x ds) a (trm_var (avar_f y)) = open_defs x ds' ->
+    G ⊢ trm_var (avar_f y) : T ->
+    G ⊢ trm_val (val_obj S ds') : typ_bnd S.
+Proof.
+  intros.
+  pick_fresh z.
+  assert (z \notin (fv_ctx_types G \u fv_defs ds \u fv_typ S)) by auto.
+  assert (z \notin L) by auto.
+  assert (G & z ~ open_typ z S /- open_defs z ds :: open_typ z S) by eauto.
+  assert (z # G) by auto.
+  assert (G ⊢ trm_var (avar_f x) : open_typ x S) by auto.
+  assert (Hdt: G /- open_defs x ds :: open_typ x S) by eauto using renaming_def.
+  clear H9 H8 H7 H6 H5.
+  pose proof (defs_update_typing H2 Hdt H4).
+  rewrite H3 in H5.
+Qed.
 
 (** [s: G]                  #<br>#
     [inert [G]              #<br>#
@@ -92,12 +222,13 @@ Lemma preservation_helper: forall G s t s' t' T,
     well_typed G s ->
     inert G ->
     (s, t) |-> (s', t') ->
-    G ⊢ t : T ->
+    ty_trm_aux G t T ->
     exists G', inert G' /\
           well_typed (G & G') s' /\
-          G & G' ⊢ t' : T.
+          ty_trm_aux (G & G') t' T.
 Proof.
   introv Hwf Hin Hred Ht. gen t'.
+  induction Ht as [? ? ? Ht | ? ? ? ? Ht | ? ? ? ? ? ? BiG Hr Ht IHt | ? ? ? ? ? ? Htt Htu | ? ? ? ? Ht Hsub].
   induction Ht; intros; try solve [invert_red; trm_val_contra].
   - Case "ty_all_intro".
     red_trm_to_val.
@@ -114,6 +245,7 @@ Proof.
       ** rewrite <- concat_empty_l. constructor~. apply (precise_inert_typ Hv).
       ** apply~ well_typed_push. apply (precise_to_general_v Hv).
       ** assert (G & x ~ V ⊢ trm_var (avar_f x) : V) by auto.
+         apply ty_aux_gen.
          eapply ty_sub. apply H2. apply* weaken_subtyp.
   - Case "ty_all_elim".
     match goal with
@@ -124,6 +256,7 @@ Proof.
     end.
     exists (@empty typ). rewrite concat_empty_r. repeat_split_right; auto.
     pick_fresh y. assert (y \notin L) as FrL by auto. specialize (Hty y FrL).
+    apply ty_aux_gen.
     eapply renaming_typ; eauto.
   - Case "ty_new_intro".
     red_trm_to_val.
@@ -140,30 +273,174 @@ Proof.
       ** rewrite <- concat_empty_l. constructor~. apply (precise_inert_typ Hv).
       ** apply~ well_typed_push. apply (precise_to_general_v Hv).
       ** assert (G & x ~ V ⊢ trm_var (avar_f x) : V) by auto.
+         apply ty_aux_gen.
          eapply ty_sub. apply H1. apply* weaken_subtyp.
   - Case "ty_new_elim".
     pose proof (canonical_forms_obj Hin Hwf Ht) as [S [ds [t [Bis [Has Ty]]]]].
     invert_red; trm_val_contra. binds_eq.
     exists (@empty typ). rewrite concat_empty_r. repeat_split_right; auto.
-    match goal with
-    | [Hd: defs_has _ (def_trm _ ?t') |- G ⊢ t': T] =>
-      rewrite* <- (defs_has_inv Has Hd)
-    end.
   - Case "ty_let".
     destruct t; try solve [solve_let].
     + SCase "[t = (let x = a in u)] where a is a variable".
       repeat invert_red; trm_val_contra.
       exists (@empty typ). rewrite concat_empty_r. repeat_split_right; auto.
+      apply ty_aux_gen.
       apply* renaming_fresh.
   - Case "ty_sub".
     solve_IH.
-    match goal with
-    | [Hs: _ ⊢ _ <: _,
-       Hg: _ & ?G' ⊢ _: _ |- _] =>
-      apply weaken_subtyp with (G2:=G') in Hs;
-      eauto
-    end.
+    eapply ty_aux_sub.
+    apply H2.
+    eapply weaken_subtyp; eauto.
+  - Case "ty_aux_force".
+    intros.
+    exists (@empty typ). rewrite concat_empty_r.
+    split; auto.
+    invert_red; trm_val_contra.
+    + split; auto.
+      pose proof (sel_to_var_typ Ht).
+      pose proof (canonical_forms_obj Hin Hwf H) as [S [ds' [t [Bis [Has Ty]]]]].
+      pose proof (binds_func H1 Bis).
+      injection H0; intros; subst.
+      pose proof (defs_has_inv H5 Has); subst t.
+      apply ty_aux_gen; auto.
+    + split; auto.
+      pose proof (sel_to_var_typ Ht).
+      pose proof (var_typ_rcd_to_binds Hin H) as [?S [?T [? [? ?]]]].
+      assert (G ⊢ trm_var (avar_f x) : typ_rcd (dec_trm a T1)) by eauto using record_has_typing.
+      pose proof (canonical_forms_obj Hin Hwf H4) as [?S [ds' [t' [Bis [Has Ty]]]]].
+      pose proof (binds_func H3 Bis).
+      injection H7; intros; subst; clear H7.
+      pose proof (defs_has_inv H5 Has); subst t'.
+      eapply ty_aux_sub.
+      eapply ty_aux_force_assgn. all: eauto.
+  - Case "ty_aux_force_assgn".
+    intros.
+    destruct t.
+    + invert_red; trm_val_contra.
+      invert_red; trm_val_contra.
+      exists (@empty typ). rewrite concat_empty_r.
+      repeat_split_right; auto.
+      split; auto.
+      destruct H0 as [? [? [? [? [?T [?ds [?ds [? [? ?]]]]]]]]].
+      split; auto.
+      split.
+      { destruct Hwf. destruct_all; congruence. }
+      intros.
+      destruct (classicT (x = x0)).
+      * subst x0. pose proof (binds_func H6 BiG).
+        subst T1.
+        pose proof (binds_func H4 H7); subst v; clear H7.
+        assert (G ⊢ trm_val (val_obj T0 ds) : typ_bnd S) by (unfold well_typed in *; destruct_all; eauto).
+        assert (G ⊢ trm_var (avar_f y) : T) by auto using var_aux_to_gen.
+
+        injection H10; intros; subst T0 ds'. clear H10 H5.
+        pose proof (binds_func H9 H6); subst v.
+      * assert (binds x0 v s) by (apply H2; auto).
+        destruct Hwf as [? [? [? ?Htv]]].
+        apply* Htv.
+
+
+
+
+      * subst x0.
+
+
+      assert (Htx: G ⊢ trm_var (avar_f x) : typ_rcd (dec_trm a T)) by eauto using record_has_typing.
+
+
+
+      pose proof (sel_to_var_typ Ht).
+      pose proof (var_typ_rcd_to_binds Hin H) as [?S [?T [? [? ?]]]].
+      assert (G ⊢ trm_var (avar_f x) : typ_rcd (dec_trm a T1)) by eauto using record_has_typing.
+      pose proof (canonical_forms_obj Hin Hwf H4) as [?S [ds' [t' [Bis [Has Ty]]]]].
+      pose proof (binds_func H3 Bis).
+      injection H7; intros; subst; clear H7.
+      pose proof (defs_has_inv H5 Has); subst t'.
+      eapply ty_aux_sub.
+      eapply ty_aux_force_assgn. all: eauto.
+
+
+
+
+
+      pose proof (sel_to_var_typ Ht).
+      pose proof (var_typ_rcd_to_binds Hin H) as [?S [?T [? [? ?]]]].
+      pose proof (canonical_forms_obj Hin Hwf H) as [?S [ds' [t [Bis [Has Ty]]]]].
+      split; auto.
+      split; try apply H0.
+      pose proof H0 as [? [? [? [? [?T [?ds [?ds [? [? ?]]]]]]]]].
+      split.
+      { destruct Hwf. destruct_all. congruence. }
+      intros.
+      destruct (classicT (x = x0)).
+      * subst x0. pose proof (binds_func H5 Bis).
+        injection H10; intros; subst T0 ds'. clear H10 H5.
+        pose proof (binds_func H9 H6); subst v.
+
+      SearchAbout (binds _ _ _).
+      Check binds_push_eq_inv.
+
+
+
+      pose proof (binds_func H1 Bis).
+      injection H0; intros; subst.
+      pose proof (defs_has_inv H5 Has); subst t.
+      apply ty_aux_gen; auto.
+    +
+
+Ltac solve_IH_assgn :=
+  match goal with
+  | [Wf: well_typed _ _,
+     In: inert _,
+     IH: well_typed _ _ ->
+         inert _ ->
+         forall t', (_, _) |-> (_, _) -> _,
+     Hr: (_, _) |-> (_, ?t') |- _] =>
+    specialize (IH Wf In t' Hr); destruct_all
+  end;
+  match goal with
+  | [Hi: _ & ?G' ⊢ _ : _ |- _] =>
+    exists G'; repeat_split_right; auto
+  | [Hi: ty_trm_aux (_ & ?G') _ _ |- _] =>
+    exists G'; repeat_split_right; auto
+  end.
+
+Ltac solve_force_assgn :=
+  invert_red; trm_val_contra; solve_IH_assgn;
+  apply ty_aux_force_assgn; eauto; apply* weaken_rules || apply* weaken_ty_aux.
+
+
+
+  invert_red; trm_val_contra.
+
+ specialize (IHHta Hwf Hin t0' H0); destruct_all.
+
+  match goal with
+  | [Wf: well_typed _ _,
+     In: inert _,
+     IH: well_typed _ _ ->
+         inert _ ->
+         forall t', (_, _) |-> (_, _) -> _,
+     Hr: (_, _) |-> (_, ?t') |- _] =>
+    (* specialize (IH Wf In t' Hr); destruct_all *)
+    idtac
+  end.
+
+  solve_IH_assgn.
+  apply ty_aux_force_assgn; eauto; apply* weaken_rules || apply* weaken_ty_aux.
+
+
+  apply ty_aux_force_assgn; eauto; apply* weaken_rules || apply* weaken_ty_aux.
+
+  invert_red; trm_val_contra; solve_IH;
+  apply ty_aux_force_assgn; eauto; apply* weaken_rules || apply* weaken_ty_aux.
+    destruct t; try solve [solve_let].
+    invert_red.
+
+    repeat_split_right; auto.
 Qed.
+  Focus 2. intros. exists (@empty typ); rewrite concat_empty_r; repeat_split_right; auto.
+  invert_red; auto. induction v; simpl in *; congruence. apply ty_aux_gen.
 
 (** ** Preservation Theorem *)
 
